invlist with_invlist (with support for effect parametric checking of with_inv, annotating opens for with_inv, etc.

pulse/src/checker/Pulse.Checker.WithInv.fst
@@ -295,17 +295,12 @@ let check
   let post_hint : post_hint_t =
     match returns_inv, post_hint with
     | None, Some post -> post
-    | Some (b, post), None ->
-      //
-      // When returns is annotated, it is annotated with only fp' (see typing rule)
-      // Adding inv i p in the post hint makes the treatment of this case,
-      //   and when post hint is coming from postcondition uniform
-      //
+    | Some (b, post, opens), None ->
       Pulse.Checker.Base.intro_post_hint g
-        (EffectAnnotAtomicOrGhost { opens = Pulse.Reflection.Util.add_inv_tm tm_emp_inames i })
+        (EffectAnnotAtomicOrGhost { opens })
         (Some b.binder_ty)
-        (tm_star (tm_inv i p) post)
-    | Some (_, post), Some q ->
+        post
+    | Some (_, post, _), Some q ->
       let open Pulse.PP in
       fail_doc g (Some t.range) 
         [ doc_of_string "Fatal: multiple annotated postconditions on with_invariant";
@@ -394,8 +389,12 @@ let check
 
   let (| body, c_body, body_typing |) =
     let ppname = mk_ppname_no_range "with_inv_body" in
+    T.print "Checking withinv body\n";
     let r = check g pre_body pre_body_typing (Some post_hint_body) ppname body in
-    apply_checker_result_k r ppname
+    T.print "Checked withinv body\n";
+    let r = apply_checker_result_k r ppname in
+    T.print "Applied checker result\n";
+    r
   in
 
   assert (comp_inames c_body == opens_remove_i);
@@ -468,7 +467,9 @@ let check
           STS_GhostInvs _ st add_inv opens tok |) in
     let d : st_typing _ _ c_out_opens =
       T_Sub _ _ _ _ d d_sub_c in
-    checker_result_for_st_typing (| _, _, d |) res_ppname
+    let r = checker_result_for_st_typing (| _, _, d |) res_ppname in
+    T.print "Returning from withinv\n";
+    r
 
   | EffectAnnotSTT ->
     let d = T_Lift _ _ _ _ d (Lift_STAtomic_ST _ c_out) in
