pulse/src/checker/Pulse.Syntax.Naming.fsti
@@ -155,9 +155,10 @@ let rec freevars_st (t:st_term)
     | Tm_WithInv { name; body; returns_inv } ->
       Set.union (Set.union (freevars name) (freevars_st body))
                 (freevars_opt 
-                  (fun (b, r) ->
+                  (fun (b, r, is) ->
                     (Set.union (freevars b.binder_ty) 
-                               (freevars r)))
+                               (Set.union (freevars r)
+                                          (freevars is))))
                   returns_inv)
 
 and freevars_branches (t:list (pattern & st_term)) : Set.set var =
@@ -345,9 +346,10 @@ let rec ln_st' (t:st_term) (i:int)
       ln' name i &&
       ln_st' body i &&
       ln_opt'
-        (fun (b, r) i ->
+        (fun (b, r, is) i ->
           ln' b.binder_ty i &&
-          ln' r (i + 1))
+          ln' r (i + 1) &&
+          ln' is i)
         returns_inv i
 
 and ln_branch' (b : pattern & st_term) (i:int) : Tot bool (decreases b) =
@@ -612,9 +614,10 @@ let rec subst_st_term (t:st_term) (ss:subst)
       let returns_inv =
         match returns_inv with
         | None -> None
-        | Some (b, r) ->
+        | Some (b, r, is) ->
           Some (subst_binder b ss, 
-                subst_term r (shift_subst ss))
+                subst_term r (shift_subst ss),
+                subst_term is ss)
       in
       Tm_WithInv { name; body; returns_inv }
 
