pulse/src/checker/Pulse.Syntax.Base.fst
@@ -264,7 +264,10 @@ let rec eq_st_term (t1 t2:st_term)
     | Tm_WithInv {name=name1; returns_inv=r1; body=body1},
       Tm_WithInv {name=name2; returns_inv=r2; body=body2} ->
       eq_tm name1 name2 &&
-      eq_opt (fun (b1, r1) (b2, r2) -> eq_tm b1.binder_ty b2.binder_ty && eq_tm r1 r2)
+      eq_opt (fun (b1, r1, is1) (b2, r2, is2) ->
+              eq_tm b1.binder_ty b2.binder_ty &&
+              eq_tm r1 r2 &&
+              eq_tm is1 is2)
              r1 r2 &&
       eq_st_term body1 body2
 
